src/StandaloneHaskellMain.v
@@ -125,20 +125,15 @@ Module WordByWordMontgomery.
     := main_gen ForExtraction.WordByWordMontgomery.PipelineMain.
 End WordByWordMontgomery.
 
-Module SaturatedSolinas.
-  Definition main : IO_unit
-    := main_gen ForExtraction.SaturatedSolinas.PipelineMain.
-End SaturatedSolinas.
-
 Module DettmanMultiplication.
   Definition main : IO_unit
     := main_gen ForExtraction.DettmanMultiplication.PipelineMain.
 End DettmanMultiplication.
 
-Module SolinasReduction.
+Module P256ADX.
   Definition main : IO_unit
-    := main_gen ForExtraction.SolinasReduction.PipelineMain.
-End SolinasReduction.
+    := main_gen ForExtraction.P256ADX.PipelineMain.
+End P256ADX.
 
 Module BaseConversion.
   Definition main : IO_unit
